stlogR.v
@@ -1,14 +1,28 @@
 Set Automatic Coercions Import.
 Require Import ssreflect ssrbool ssrnat eqtype seq ssrfun.
-Require Import pred pcm unionmap heap heaptac stmod stsep stlog. 
+Require Import pred prelude pcm unionmap heap heaptac stmod stsep stlog. 
 Set Implicit Arguments.
 Unset Strict Implicit.
 Import Prenex Implicits.
 
-(**********************************************************)
-(* First, the reflection mechanism for search-and-replace *)
-(* pattern-matching on heap expressions.                  *)
-(**********************************************************)
+(**************************************************************************)
+(* This file implements two different automations related to Hoare logic. *)
+(*                                                                        *)
+(* First automation concerns selection of Hoare-style rule for symbolic   *)
+(* evaluation. The first command of the program determines the applicable *)
+(* rule uniquely. The implemented automation picks out this rule, and     *)
+(* applies it, while using AC-theory of heaps to rearrange the goal, if   *)
+(* necessary for the rule to apply.                                       *)
+(*                                                                        *)
+(* Second automation concerns pulling ghost variables out of a Hoare      *)
+(* type. The non-automated lemmas do this pulling one variable at a       *)
+(* time. The automation pulls all the variable at once.                   *)
+(**************************************************************************)
+
+(****************************************************************)
+(* First, the reflection mechanism for search-and-replace       *)
+(* pattern-matching on heap expressions; the AC theory of heaps *)
+(****************************************************************)
 
 Structure tagged_heap := Tag {untag :> heap}.
 
@@ -46,9 +60,9 @@ Proof. by rewrite formE /form_axiom /= joinCA. Qed.
 Canonical Structure search_right h r (f : forall k, form k r) k := 
   Form k (h \+ r) (right_tag (h \+ f k)) (right_pf h f k).
 
-(*********************)
-(* Reflective lemmas *)
-(*********************)
+(**********************************************************)
+(* Reflective lemmas that apply module AC-theory of heaps *)
+(**********************************************************)
 
 Notation cont A := (ans A -> heap -> Prop).
 
@@ -315,6 +329,67 @@ Canonical Structure bnd_dealloc_form A B s v x r j f :=
   BndForm (@bnd_deallocR A B s v x j f r).
 Canonical Structure try_dealloc_form A B s1 s2 v x r j f := 
   TryForm (@try_deallocR A B s1 s2 v x j f r).
+
+(* Second automation *)
+
+(**************************************************************************)
+(* A simple canonical structure program to automate applying ghE and gh.  *)
+(*                                                                        *)
+(* The gh_form pivots on a spec, and computes as output the following.    *)
+(* - rT is a product of types of all encounted ghost vars.                *)
+(* - p and q are pre and post parametrized by rT that should be output by *)
+(*   the main lemma.                                                      *)
+(*                                                                        *)
+(* In the future, rT should be a list of types, rather than a product,    *)
+(* but that leads to arity polimorphism, and dependent programming, which *)
+(* I want to avoid for now.                                               *)
+(**************************************************************************)
+
+Section Automation.
+Structure tagged_spec A := gh_step {gh_untag :> spec A}.
+Canonical Structure gh_base A (s : spec A) := gh_step s.
+
+Definition gh_axiom A rT p q (pivot : tagged_spec A) := 
+  gh_untag pivot = logvar (fun x : rT => binarify (p x) (q x)).
+
+Structure gh_form A rT (p : rT -> pre) (q : rT -> cont A) := GhForm {
+   gh_pivot :> tagged_spec A;
+   _ : gh_axiom p q gh_pivot}. 
+
+(* the main lemma that automates the applications of ghE and gh *)
+
+Lemma ghR A e rT p q (f : @gh_form A rT p q) : 
+        (forall i x, p x i -> valid i -> verify i e (q x)) ->
+        conseq e f. 
+Proof. by case: f=>p' ->; apply: gh. Qed.
+
+(* base case; check if we reached binarify *)
+
+Lemma gh_base_pf A rT (p : rT -> pre) (q : rT -> cont A) :
+        gh_axiom p q (gh_base (logvar (fun x => binarify (p x) (q x)))).
+Proof. by []. Qed.
+
+Canonical gh_base_struct A rT p q := GhForm (@gh_base_pf A rT p q).
+                 
+(* inductive case; merge adjacent logvars and continue *)
+
+Lemma gh_step_pf A B rT p q (f : forall x : A, @gh_form B rT (p x) (q x)) : 
+        gh_axiom (fun xy => p xy.1 xy.2) (fun xy => q xy.1 xy.2)
+                 (gh_step (logvar (fun x => f x))).
+Proof. 
+congr (_, _).
+- apply: fext=>i; apply: pext; split. 
+  - by case=>x; case: (f x)=>[_ ->] /= [y H]; exists (x, y). 
+  by case; case=>x y; exists x; case: (f x)=>[_ ->]; exists y.  
+apply: fext=>y; apply: fext=>i; apply: fext=>m; apply: pext; split.
+- by move=>H [x z] /= H1; case: (f x) (H x)=>[_ ->]; apply.  
+by move=>H x; case: (f x)=>[_ ->] z; apply: (H (x, z)).
+Qed.
+
+Canonical gh_step_struct A B rT p q f := GhForm (@gh_step_pf A B rT p q f). 
+
+End Automation.
+
 
 (* we keep some tactics to kill final goals, which *)
 (* are usually full of existentials *)
